lean/dk_math/DkMath/Collatz/PetalBridge/FloatWindow.lean
@@ -20,6 +20,7 @@ import DkMath.Collatz.PetalBridge.FloatWindow.UniversalPaymentRepayment
 import DkMath.Collatz.PetalBridge.FloatWindow.UniversalPaymentDepthLedger
 import DkMath.Collatz.PetalBridge.FloatWindow.UniversalPaymentScalarQueue
 import DkMath.Collatz.PetalBridge.FloatWindow.UniversalPaymentBlockNormalForm
+import DkMath.Collatz.PetalBridge.FloatWindow.UniversalPaymentPositiveBlock
 import DkMath.Collatz.PetalBridge.FloatWindow.UniversalPaymentPrimitiveExcursion
 import DkMath.Collatz.PetalBridge.FloatWindow.FiniteSignedTransition
 
